qsort/verif_qsort3.v
@@ -1,0 +1,1751 @@
+Require Import VST.floyd.proofauto.
+Require Import qsort3.
+Instance CompSpecs : compspecs. make_compspecs prog. Defined.
+Definition Vprog : varspecs. mk_varspecs prog. Defined.
+
+Require Import float_lemmas.
+Require Import Permutation.
+
+Definition quicksort_spec :=
+ DECLARE _quicksort
+  WITH base: val, N: Z, al: list val
+  PRE  [ _base_ptr OF tptr tdouble, _total_elems OF tint] 
+    PROP(N=Zlength al; N <=Z.min Int.max_signed (Ptrofs.max_signed / sizeof tdouble); Forall def_float al)
+    LOCAL(temp _base_ptr base; temp _total_elems (Vint (Int.repr N)))
+    SEP(data_at Ews (tarray tdouble N) al base)
+  POST [ tvoid ]
+    EX bl: list val,
+     PROP(Permutation al bl; sorted (f_cmp Cle) bl) 
+     LOCAL ()
+    SEP(data_at Ews (tarray tdouble N) bl base).
+
+Definition main_spec :=
+ DECLARE _main
+  WITH gv : globals
+  PRE  [] main_pre prog nil gv
+  POST [ tint ]  
+     PROP() 
+     LOCAL (temp ret_temp (Vint (Int.repr 0)))
+     SEP(TT).
+
+Definition Gprog : funspecs :=
+        ltac:(with_library prog [quicksort_spec]).
+
+Set Nested Proofs Allowed.
+
+Lemma no_saturate_hack:
+  forall sh n al p,
+    data_at sh (tarray tdouble n) al p |-- !!True.
+Proof.
+intros. apply prop_right. auto.
+Qed.
+(*Hint Resolve no_saturate_hack: saturate_local. *)
+
+Definition dnth (a: val) (i: Z) : val :=
+   eval_binop Oadd (tptr tdouble) tint a (Vint (Int.repr i)).
+
+Lemma data_at_tarray_weak_valid_pointer {CS: compspecs}:
+  forall sh t n cts b z i,
+   sepalg.nonidentity sh ->
+   0 < n <= Int.max_signed->
+   0 < sizeof t ->
+   0 <= i <= n ->
+   data_at sh (tarray t n) cts (Vptr b z) |--
+   weak_valid_pointer (Vptr b (Ptrofs.add z (Ptrofs.mul (Ptrofs.repr (sizeof t))
+                                      (Ptrofs.of_ints (Int.repr i))))).
+Proof.
+intros.
+eapply derives_trans; [apply data_at_memory_block |].
+eapply derives_trans; [apply memory_block_weak_valid_pointer |]; auto.
+instantiate (1:= (i * sizeof t)%Z).
+split.
+apply Z.mul_nonneg_nonneg; try omega.
+simpl sizeof.
+rewrite Z.max_r by omega.
+rewrite Z.mul_comm.
+apply Z.mul_le_mono_nonneg_l; try omega.
+simpl.
+rewrite Z.max_r by omega.
+apply Z.mul_pos_pos; try omega.
+apply derives_refl'.
+f_equal.
+simpl.
+f_equal.
+f_equal.
+normalize.
+f_equal.
+apply Z.mul_comm.
+Qed.
+
+Lemma data_at_tarray_valid_pointer {CS: compspecs}:
+  forall sh t n cts b z i,
+   sepalg.nonidentity sh ->
+   0 < n <= Int.max_signed->
+   0 < sizeof t ->
+   0 <= i < n ->
+   data_at sh (tarray t n) cts (Vptr b z) |--
+   valid_pointer (Vptr b (Ptrofs.add z (Ptrofs.mul (Ptrofs.repr (sizeof t))
+                                      (Ptrofs.of_ints (Int.repr i))))).
+Proof.
+intros.
+eapply derives_trans; [apply data_at_memory_block |].
+eapply derives_trans; [apply memory_block_valid_pointer |]; auto.
+instantiate (1:= (i * sizeof t)%Z).
+split.
+apply Z.mul_nonneg_nonneg; try omega.
+simpl sizeof.
+rewrite Z.max_r by omega.
+rewrite  (Z.mul_comm i).
+apply Zmult_lt_compat_l; omega.
+simpl offset_val.
+apply derives_refl'.
+f_equal.
+f_equal.
+f_equal.
+normalize.
+f_equal.
+apply Z.mul_comm.
+Qed.
+
+Lemma test_order_dnth:
+  forall N (bl: list val) base lo hi,
+   0 < N <= Int.max_signed ->
+   0 <= lo <= N ->
+   0 <= hi <= N ->
+   Zlength bl = N ->
+  data_at Ews (tarray tdouble N) bl base
+    |-- denote_tc_test_order (dnth base lo) (dnth base hi).
+Proof.
+intros.
+entailer!.
+unfold dnth.
+make_Vptr base.
+simpl.
+unfold test_order_ptrs.
+simpl.
+destruct (peq b b);[ | congruence].
+simpl. clear e.
+apply andp_right.
+apply data_at_tarray_weak_valid_pointer; auto.
+compute; auto.
+apply data_at_tarray_weak_valid_pointer; auto.
+compute; auto.
+Qed.
+
+Hint Resolve test_order_dnth: valid_pointer.
+
+Lemma test_eq_dnth:
+  forall N (bl: list val) base lo hi,
+   0 < N <= Int.max_signed ->
+   0 <= lo < N ->
+   0 <= hi < N ->
+   Zlength bl = N ->
+  data_at Ews (tarray tdouble N) bl base
+    |-- denote_tc_test_eq (dnth base lo) (dnth base hi).
+Proof.
+intros.
+entailer!.
+unfold dnth.
+make_Vptr base.
+simpl eval_binop.
+apply denote_tc_test_eq_split.
+apply data_at_tarray_valid_pointer; auto.
+compute; auto.
+apply data_at_tarray_valid_pointer; auto.
+compute; auto.
+Qed.
+
+Hint Resolve test_eq_dnth: valid_pointer.
+
+Lemma isptr_dnth: forall base i, isptr base -> isptr (dnth base i).
+Proof.
+intros.
+unfold dnth.
+make_Vptr base; simpl.
+auto.
+Qed.
+Hint Resolve isptr_dnth.
+
+Lemma denote_tc_samebase_dnth:
+  forall P base i j,  
+   isptr base ->
+   P |-- denote_tc_samebase (dnth base i) (dnth base j).
+Proof.
+intros.
+make_Vptr base.
+unfold dnth, denote_tc_samebase; unfold sameblock; simpl.
+unfold peq.
+apply prop_right.
+destruct (Pos.eq_dec b b); simpl; auto.
+Qed.
+Hint Resolve denote_tc_samebase_dnth.
+
+Definition quicksort_while_body := 
+match fn_body f_quicksort with
+Ssequence _ (Ssequence _ (Ssequence _ (Sloop (Ssequence _ body) _))) =>
+body
+| _ => Sskip
+end.
+
+Lemma mid_in_range:
+   forall lo hi: Z, lo < hi -> lo <= lo + (hi-lo)/2 < hi.
+Proof.
+intros.
+assert (0 < (hi-lo)) by omega.
+assert (0 <= (hi-lo)/2 < (hi-lo)); [ | omega].
+clear H.
+forget (hi-lo) as i.
+split.
+apply Z.div_pos; omega.
+apply Z.div_lt_upper_bound; try omega.
+Qed.
+
+Lemma dnth_base_field_address:
+ forall base i N, 
+    field_compatible (tarray tdouble N) [] base ->
+    0 <= i < N ->
+    dnth base i = field_address (tarray tdouble N) [ArraySubsc i] base.
+Proof.
+intros.
+make_Vptr base. 
+unfold field_address, dnth.
+rewrite if_true.
+simpl.
+normalize.
+f_equal. f_equal.
+f_equal.
+f_equal.
+destruct H as [_ [_ [? _]]].
+red in H.
+simpl sizeof in H.
+rewrite Z.max_r in H by omega.
+apply Int.signed_repr.
+rep_omega.
+destruct H as [? [? [? [? ?]]]].
+split3; auto.
+split3; auto.
+hnf.
+split; auto.
+Qed.
+
+Lemma dnth_base_field_address0:
+ forall base i N, 
+    field_compatible (tarray tdouble N) [] base ->
+    0 <= i <= N ->
+    dnth base i = field_address0 (tarray tdouble N) [ArraySubsc i] base.
+Proof.
+intros.
+make_Vptr base. 
+unfold field_address0, dnth.
+rewrite if_true.
+simpl.
+normalize.
+f_equal. f_equal.
+f_equal.
+f_equal.
+destruct H as [_ [_ [? _]]].
+red in H.
+simpl sizeof in H.
+rewrite Z.max_r in H by omega.
+apply Int.signed_repr.
+rep_omega.
+destruct H as [? [? [? [? ?]]]].
+split3; auto.
+split3; auto.
+hnf.
+split; auto.
+Qed.
+
+Lemma typed_true_cmp:
+  forall op x y,
+    typed_true tint
+        (force_val
+           (both_float
+              (fun n1 n2 : float =>
+               Some (Val.of_bool (Float.cmp op n1 n2)))
+              sem_cast_f2f sem_cast_f2f 
+              x y)) ->
+   f_cmp op x y.
+Proof.
+intros.
+destruct x,y; simpl in H; try solve [inv H].
+hnf in H.
+unfold f_cmp.
+destruct (Float.cmp op f f0); auto. inv H.
+Qed.
+
+Lemma typed_false_cmp:
+  forall op x y,
+    def_float x -> def_float y ->
+    typed_false tint
+        (force_val
+           (both_float
+              (fun n1 n2 : float =>
+               Some (Val.of_bool (Float.cmp op n1 n2)))
+              sem_cast_f2f sem_cast_f2f 
+              x y)) ->
+   f_cmp (negate_comparison op) x y.
+Proof.
+intros.
+destruct x,y; simpl in H1; try solve [inv H1].
+apply f_cmp_false; auto.
+destruct (Float.cmp op f f0); auto. inv H1.
+Qed.
+
+Lemma Permutation_Zlength:
+  forall {A} {al bl: list A}, Permutation al bl -> Zlength al = Zlength bl.
+Proof.
+intros. rewrite !Zlength_correct. f_equal. apply Permutation_length; auto.
+Qed.
+
+Definition swap_in_list {A}{INa: Inhabitant A} i j (bl: list A) :=
+  (upd_Znth i (upd_Znth j bl (Znth i bl)) (Znth j bl)).
+
+Lemma Forall_swap_in_list {A}{INa: Inhabitant A}:
+  forall i j (bl: list A) (P: A -> Prop),
+  0 <= i < Zlength bl ->
+  0 <= j < Zlength bl ->
+  Forall P bl ->
+  Forall P (swap_in_list i j bl).
+Proof.
+intros.
+unfold swap_in_list.
+rewrite !upd_Znth_unfold.
+rewrite !Forall_app.
+split3.
+apply Forall_sublist. 
+rewrite !Forall_app.
+split3.
+apply Forall_sublist; auto.
+rewrite <- sublist_len_1 by omega.
+apply Forall_sublist; auto.
+apply Forall_sublist; auto.
+rewrite <- sublist_len_1 by omega.
+apply Forall_sublist; auto.
+apply Forall_sublist.
+rewrite !Forall_app.
+split3.
+apply Forall_sublist; auto.
+rewrite <- sublist_len_1 by omega.
+apply Forall_sublist; auto.
+apply Forall_sublist; auto.
+Qed.
+
+Lemma Permutation_swap2:
+  forall {A}{INa: Inhabitant A} lo mid (bl: list A),
+    0 <= lo < Zlength bl ->
+    0 <= mid < Zlength bl ->
+    lo <> mid ->
+    Permutation bl (swap_in_list lo mid bl).
+Proof.
+intros.
+  unfold swap_in_list.
+  set (N := Zlength bl) in *.
+  rewrite !upd_Znth_unfold.
+  autorewrite with sublist.
+ replace  (mid + (Z.succ 0 + (Zlength bl - (mid + 1))))
+    with N by omega.
+  destruct (zlt lo mid).
+  rewrite (sublist_split (lo+1) mid N) by list_solve.
+  autorewrite with sublist.
+  rewrite (sublist_app 0 (N-mid)) by list_solve.
+  autorewrite with sublist.
+  replace (N - mid - Z.succ 0 + (mid + 1)) with N by omega.
+  rewrite (sublist_one 0 (Z.succ 0)) by list_solve.
+  autorewrite with sublist.
+  erewrite <- !sublist_len_1 by list_solve. 
+  apply Permutation_trans 
+   with (sublist 0 lo bl ++
+    sublist lo (lo + 1) bl ++
+   sublist (lo + 1) mid bl ++
+   sublist mid (mid + 1) bl ++ sublist (mid + 1) N bl).
+   autorewrite with sublist. apply Permutation_refl.
+   apply Permutation_app_head.
+   rewrite <- !app_ass.
+   apply Permutation_app_tail.
+  eapply Permutation_trans; [apply Permutation_app_comm |].
+   rewrite !app_ass.
+   apply Permutation_app_head.
+   apply Permutation_app_comm.
+   rewrite (sublist_app2 (lo+1) N) by list_solve.
+   autorewrite with sublist.
+   rewrite (sublist_app2 (lo+1-mid)) by list_solve.
+   autorewrite with sublist.
+   replace (lo + 1 - mid - Z.succ 0 + (mid + 1)) with (lo+1) by omega.
+  rewrite (sublist_app 0 lo); try list_solve.
+  autorewrite with sublist.
+  replace (N - mid - Z.succ 0 + (mid + 1)) with N by omega.
+  rewrite sublist_app by list_solve.
+  rewrite Z.min_l by rep_omega.
+  autorewrite with sublist.
+  rewrite (sublist_one 0 (Z.succ 0)) by list_solve.
+  autorewrite with sublist.
+  replace (lo - mid - Z.succ 0 + (mid + 1)) with lo by omega.
+  erewrite <- !sublist_len_1 by list_solve.
+  apply Permutation_trans 
+   with (sublist 0 mid bl ++
+    sublist mid (mid + 1) bl ++
+   sublist (mid + 1) lo bl ++
+   sublist lo (lo + 1) bl ++ sublist (lo + 1) N bl).
+   autorewrite with sublist. apply Permutation_refl.
+   rewrite !app_ass.
+   apply Permutation_app_head.
+   rewrite <- !app_ass.
+   apply Permutation_app_tail.
+  eapply Permutation_trans; [apply Permutation_app_comm |].
+   rewrite !app_ass.
+   apply Permutation_app_head.
+   apply Permutation_app_comm.
+Qed.
+
+Definition quicksort_while_body_part2 := 
+match quicksort_while_body
+  with Ssequence _ (Ssequence _ (Ssequence _ a)) =>
+     a
+| _ => Sskip
+end.
+
+Lemma dbase_sub:
+ forall  base i j,
+  isptr base -> 
+  Int.min_signed <= i <= Int.max_signed ->
+  Int.min_signed <= j <= Int.max_signed ->
+  Int.min_signed <= i-j <= Int.max_signed ->
+   (force_val
+               (sem_binary_operation' Osub 
+                  (tptr tdouble) tint (dnth base i)
+                  (Vint (Int.repr j)))) =
+   (dnth base (i-j)).
+Proof.
+intros.
+unfold dnth.
+make_Vptr base.
+simpl.
+f_equal.
+rewrite Ptrofs.sub_add_opp.
+rewrite Ptrofs.add_assoc. f_equal.
+normalize.
+rewrite Ptrofs.neg_repr.
+normalize. f_equal. rewrite Z.add_opp_r.
+rewrite <- Z.mul_sub_distr_l.
+auto.
+Qed.
+
+Lemma dbase_add:
+ forall  base i j,
+  isptr base -> 
+  Int.min_signed <= i <= Int.max_signed ->
+  Int.min_signed <= j <= Int.max_signed ->
+  Int.min_signed <= i+j <= Int.max_signed ->
+   (force_val
+               (sem_binary_operation' Oadd 
+                  (tptr tdouble) tint (dnth base i)
+                  (Vint (Int.repr j)))) =
+   (dnth base (i+j)).
+Proof.
+intros.
+unfold dnth.
+make_Vptr base.
+simpl.
+f_equal.
+rewrite Ptrofs.add_assoc. f_equal.
+normalize.
+rewrite <- Z.mul_add_distr_l.
+auto.
+Qed.
+
+Lemma tc_val_tdouble_Znth:
+ forall Delta P Q i base N (bl: list val),
+  N = Zlength bl ->
+  0 <= i < N -> 
+  Forall def_float bl ->
+  dnth base i = field_address (tarray tdouble N) [ArraySubsc i] base ->
+  ENTAIL Delta, PROPx P (LOCALx Q (SEP (data_at Ews (tarray tdouble N) bl base)))
+    |-- local (liftx (tc_val tdouble (Znth i bl))).
+Proof.
+intros.
+go_lowerx.
+clear H4 H5.
+apply prop_right.
+change (@reptype CompSpecs tdouble) with val in *.
+apply Forall_Znth with (i0:=i) in H1; auto.
+destruct (Znth i bl); inv H1; simpl; auto.
+omega.
+Qed.
+
+Lemma typed_true_pp:
+  forall op i j N base,
+    0 < N <= Z.min Int.max_signed (Ptrofs.max_signed / 8) ->
+    dnth base i =
+      field_address (tarray tdouble N) [ArraySubsc i] base ->
+    dnth base j =
+      field_address (tarray tdouble N) [ArraySubsc j] base ->
+    typed_true tint (force_val (
+           sem_cmp_pp op (dnth base i) (dnth base j))) ->
+    Zcmp op i j.
+Proof.
+intros *. pose proof I. pose proof I. intros.
+rewrite H2,H3 in H4; clear H2 H3.
+unfold field_address in H4.
+if_tac in H4; [ | inv H4].
+if_tac in H4; [ | destruct base; inv H4].
+destruct base; try solve [inv H4].
+unfold sem_cmp_pp in H4.
+destruct Archi.ptr64 eqn: Hp; try solve [inv H4].
+simpl force_val in H4.
+rewrite if_true in H4 by auto.
+simpl force_val in H4.
+apply typed_true_of_bool in H4.
+normalize in H4.
+clear H H0.
+destruct H2 as [_ [_ [H2 [_ [_ ?]]]]].
+destruct H3 as [_ [_ [_ [_ [_ ?]]]]].
+simpl in H, H0.
+set (M := Z.min _ _) in H1; compute in M; subst M.
+simpl in H2.
+rewrite Z.max_r in H2 by omega.
+rewrite <- (Ptrofs.repr_unsigned i0) in H4.
+unfold Ptrofs.cmpu in H4.
+unfold Ptrofs.eq, Ptrofs.ltu in H4.
+normalize in H4.
+destruct op; simpl; if_tac in H4; inv H4;
+rewrite !Ptrofs.unsigned_repr in H3 by rep_omega;
+omega.
+Qed.
+
+Lemma typed_false_pp:
+  forall op i j N base,
+    0 < N <= Z.min Int.max_signed (Ptrofs.max_signed / 8) ->
+    dnth base i =
+      field_address (tarray tdouble N) [ArraySubsc i] base ->
+    dnth base j =
+      field_address (tarray tdouble N) [ArraySubsc j] base ->
+    typed_false tint (force_val (
+           sem_cmp_pp op (dnth base i) (dnth base j))) ->
+    Zcmp (negate_comparison op) i j.
+Proof.
+intros *. pose proof I. pose proof I. intros.
+rewrite H2,H3 in H4; clear H2 H3.
+unfold field_address in H4.
+if_tac in H4; [ | inv H4].
+if_tac in H4; [ | destruct base; inv H4].
+destruct base; try solve [inv H4].
+unfold sem_cmp_pp in H4.
+destruct Archi.ptr64 eqn: Hp; try solve [inv H4].
+simpl force_val in H4.
+rewrite if_true in H4 by auto.
+simpl force_val in H4.
+apply typed_false_of_bool in H4.
+normalize in H4.
+clear H H0.
+destruct H2 as [_ [_ [H2 [_ [_ ?]]]]].
+destruct H3 as [_ [_ [_ [_ [_ ?]]]]].
+simpl in H, H0.
+set (M := Z.min _ _) in H1; compute in M; subst M.
+simpl in H2.
+rewrite Z.max_r in H2 by omega.
+rewrite <- (Ptrofs.repr_unsigned i0) in H4.
+unfold Ptrofs.cmpu in H4.
+unfold Ptrofs.eq, Ptrofs.ltu in H4.
+normalize in H4.
+destruct op; simpl; if_tac in H4; inv H4;
+rewrite !Ptrofs.unsigned_repr in H3 by rep_omega;
+omega.
+Qed.
+
+Ltac pose_dnth_base i :=
+ match goal with |- 
+    semax _ (PROPx _ (LOCALx _ 
+      (SEP (data_at _ (tarray tdouble ?N) _ ?base)))) _ _ =>
+assert_PROP (dnth base i = field_address (tarray tdouble N) [ArraySubsc i] base)
+     by (entailer!; apply dnth_base_field_address; auto; omega)
+end.
+
+Lemma Znth_swap_in_list1 {A}{INH: Inhabitant A}:
+  forall i j bl, 
+  0 <= i < Zlength bl ->
+  0 <= j < Zlength bl ->
+  Znth i (swap_in_list i j bl) = Znth j bl.
+Proof.
+intros.
+unfold swap_in_list.
+rewrite upd_Znth_same by list_solve. auto.
+Qed.
+
+Lemma Znth_swap_in_list2 {A}{INH: Inhabitant A}:
+  forall i j bl, 
+  0 <= i < Zlength bl ->
+  0 <= j < Zlength bl ->
+  Znth j (swap_in_list i j bl) = Znth i bl.
+Proof.
+intros.
+unfold swap_in_list.
+destruct (zeq i j).
+subst.
+rewrite upd_Znth_same by list_solve. auto.
+rewrite upd_Znth_diff by list_solve.
+rewrite upd_Znth_same by list_solve. auto.
+Qed.
+
+Lemma Znth_swap_in_list_other {A}{INH: Inhabitant A}:
+  forall i j k bl, 
+  0 <= i < Zlength bl ->
+  0 <= j < Zlength bl ->
+  0 <= k < Zlength bl ->
+  k <> i ->
+  k <> j ->
+  Znth k (swap_in_list i j bl) = Znth k bl.
+Proof.
+intros.
+unfold swap_in_list.
+rewrite !upd_Znth_diff by list_solve.
+auto.
+Qed.
+
+Lemma sublist_swap_in_list {A}{INH: Inhabitant A}:
+  forall lo hi i j bl, 
+  0 <= lo <= hi -> 
+  hi <= Zlength bl ->
+  0 <= i < Zlength bl -> 
+  0 <= j < Zlength bl -> 
+  ~ (lo <= i < hi) ->
+  ~ (lo <= j < hi) ->
+  sublist lo hi (swap_in_list i j bl) = sublist lo hi bl.
+Proof.
+intros.
+unfold swap_in_list.
+rewrite upd_Znth_unfold.
+destruct (zle hi i).
+rewrite sublist_app1 by (autorewrite with sublist; omega).
+rewrite sublist_sublist by omega.
+rewrite upd_Znth_unfold.
+destruct (zle hi j).
+rewrite sublist_app1 by (autorewrite with sublist; omega).
+rewrite sublist_sublist by omega.
+f_equal; omega.
+rewrite sublist_app2 by  (autorewrite with sublist; omega).
+autorewrite with sublist.
+f_equal; omega.
+rewrite sublist_app2 by  (autorewrite with sublist; omega).
+autorewrite with sublist.
+rewrite upd_Znth_unfold.
+destruct (zle hi j).
+rewrite sublist_app1 by (autorewrite with sublist; omega).
+rewrite sublist_sublist by omega.
+f_equal; omega.
+rewrite sublist_app2 by  (autorewrite with sublist; omega).
+autorewrite with sublist.
+f_equal; omega.
+Qed.
+
+Lemma sublist_swap_in_list' {A}{INH: Inhabitant A}:
+ forall lo hi i j bl, 
+  i < hi ->
+  j < hi ->
+  0 <= lo <= i ->
+  0 <= lo <= j ->
+  hi <= Zlength bl ->
+  sublist lo hi (swap_in_list i j bl) = 
+  swap_in_list (i-lo) (j-lo) (sublist lo hi bl).
+Proof.
+intros.
+unfold swap_in_list.
+rewrite upd_Znth_unfold.
+rewrite sublist_app by (autorewrite with sublist; rep_omega).
+autorewrite with sublist.
+rewrite upd_Znth_unfold.
+rewrite sublist_app by (autorewrite with sublist; rep_omega).
+autorewrite with sublist.
+rewrite upd_Znth_unfold.
+destruct (zlt i j); [ | destruct (zeq i j)].
+-
+rewrite Z.min_l by omega.
+rewrite Z.max_r by omega.
+rewrite sublist_app by (autorewrite with sublist; rep_omega).
+autorewrite with sublist.
+rewrite upd_Znth_unfold.
+rewrite sublist_app by (autorewrite with sublist; rep_omega).
+autorewrite with sublist.
+rewrite sublist_app by (autorewrite with sublist; rep_omega).
+autorewrite with sublist.
+rewrite sublist_app by (autorewrite with sublist; rep_omega).
+autorewrite with sublist.
+rewrite <- !sublist_len_1 by omega.
+autorewrite with sublist.
+replace (Z.succ 0 + j) with (j+1) by (clear; omega).
+f_equal.
+f_equal.
+rewrite sublist_app by (autorewrite with sublist; rep_omega).
+autorewrite with sublist.
+replace (i-lo+1+lo) with (i+1) by omega.
+f_equal.
+rewrite sublist_app by (autorewrite with sublist; rep_omega).
+autorewrite with sublist.
+f_equal.
+f_equal. omega. omega.
+-
+subst.
+autorewrite with sublist.
+rewrite sublist_app by (autorewrite with sublist; rep_omega).
+autorewrite with sublist.
+rewrite upd_Znth_unfold.
+rewrite sublist_app by (autorewrite with sublist; rep_omega).
+autorewrite with sublist.
+rewrite <- !sublist_len_1 by omega.
+autorewrite with sublist.
+f_equal. omega.
+-
+rewrite Z.min_r by omega.
+rewrite Z.max_l by omega.
+rewrite sublist_app by (autorewrite with sublist; rep_omega).
+autorewrite with sublist.
+rewrite upd_Znth_unfold.
+rewrite sublist_app by (autorewrite with sublist; rep_omega).
+autorewrite with sublist.
+rewrite <- !sublist_len_1 by omega.
+autorewrite with sublist.
+rewrite sublist_app by (autorewrite with sublist; rep_omega).
+autorewrite with sublist.
+rewrite sublist_app by (autorewrite with sublist; rep_omega).
+autorewrite with sublist.
+rewrite !app_ass.
+f_equal.
+f_equal.
+f_equal.
+f_equal; omega.
+f_equal.
+f_equal. omega.
+f_equal; omega.
+Qed.
+
+Definition quicksort_do_loop := 
+match quicksort_while_body_part2
+  with Ssequence _ (Ssequence _ (Ssequence a _)) =>
+     a
+| _ => Sskip
+end.
+
+Lemma forward_quicksort_do_loop :
+forall (Espec : OracleKind) (base : val) (al : list val) 
+  (lo mid hi : Z) (bl : list val),
+Forall def_float al ->
+let N := Zlength al in
+0 < N <= Z.min Int.max_signed (Ptrofs.max_signed / 8) ->
+isptr base ->
+0 <= lo <= mid ->
+mid < hi < N ->
+f_cmp Cge (Znth mid bl) (Znth lo bl) ->
+f_cmp Cle (Znth mid bl) (Znth hi bl) ->
+Permutation al bl ->
+sorted (f_cmp Cle) (sublist 0 lo bl) ->
+sorted (f_cmp Cle) (sublist (hi + 1) N bl) ->
+(0 < lo ->
+ Forall (f_cmp Cle (Znth (lo - 1) bl)) (sublist lo N bl)) ->
+(hi + 1 < N ->
+ Forall (f_cmp Cge (Znth (hi + 1) bl))
+   (sublist 0 (hi + 1) bl)) ->
+
+semax (func_tycontext f_quicksort Vprog Gprog [])
+  (PROP ()
+   LOCAL (temp _right_ptr (dnth base (hi - 1));
+   temp _left_ptr (dnth base (lo + 1));
+   temp _mid (dnth base mid); temp _lo (dnth base lo);
+   temp _hi (dnth base hi))
+   SEP (data_at Ews (tarray tdouble N) bl base))
+  quicksort_do_loop
+ (normal_ret_assert 
+   (EX left:Z, EX mid:Z, EX right:Z, EX bl: list val,
+    PROP (lo < left; right < hi; lo <= mid < hi;
+       (left=right+1 \/ left=right+2)%Z;
+       Forall (f_cmp Cge (Znth mid bl)) (sublist lo left bl);
+       Forall (f_cmp Cle (Znth mid bl)) (sublist (right+1) (hi+1) bl);
+       Permutation al bl;
+       sorted (f_cmp Cle) (sublist 0 lo bl);
+       sorted (f_cmp Cle) (sublist (hi + 1) N bl);
+       0 < lo -> Forall (f_cmp Cle (Znth (lo - 1) bl)) (sublist lo N bl);
+       hi + 1 < N -> Forall (f_cmp Cge (Znth (hi + 1) bl))  (sublist 0 (hi + 1) bl))
+    LOCAL (temp _right_ptr (dnth base right);
+       temp _left_ptr (dnth base left);
+       temp _mid (dnth base mid); temp _lo (dnth base lo);
+       temp _hi (dnth base hi))
+   SEP (data_at Ews (tarray tdouble N) bl base))).
+Proof.
+intros.
+set (s := quicksort_do_loop); hnf in s; subst s.
+abbreviate_semax.
+set (M := Z.min _ _) in H0; compute in M; subst M.
+forward_loop  (EX left:Z, EX right:Z, EX bl: list val, 
+   PROP (
+   lo < left <= right+1; right < hi;
+   Forall (f_cmp Cge (Znth mid bl)) (sublist lo left bl);
+   Forall (f_cmp Cle (Znth mid bl)) (sublist (right+1) (hi+1) bl);
+   Permutation al bl;
+   sorted (f_cmp Cle) (sublist 0 lo bl);
+   sorted (f_cmp Cle) (sublist (hi + 1) N bl);
+   0 < lo -> Forall (f_cmp Cle (Znth (lo - 1) bl)) (sublist lo N bl);
+   hi + 1 < N -> Forall (f_cmp Cge (Znth (hi + 1) bl))  (sublist 0 (hi + 1) bl))
+   LOCAL (temp _left_ptr (dnth base left);
+   temp _right_ptr (dnth base right);
+   temp _mid (dnth base mid); temp _lo (dnth base lo);
+   temp _hi (dnth base hi))
+   SEP (data_at Ews (tarray tdouble N) bl base)).
+-
+Exists (lo+1) (hi-1) bl.
+entailer!.
+rewrite !sublist_one by rep_omega.
+repeat constructor.
+rewrite Z.sub_add.
+auto.
+-
+clear dependent bl.
+Intros left right bl.
+assert (Hdef_bl: Forall def_float bl) by (apply Forall_perm with al; auto).
+assert (Hlen := Permutation_Zlength H8).
+forward_loop (EX left:Z,
+   PROP (
+   lo < left <= right+1; right < hi;
+   Forall (f_cmp Cge (Znth mid bl)) (sublist lo left bl);
+   Forall (f_cmp Cle (Znth mid bl)) (sublist (right+1) (hi+1) bl);
+   Permutation al bl;
+   sorted (f_cmp Cle) (sublist 0 lo bl);
+   sorted (f_cmp Cle) (sublist (hi + 1) N bl);
+   0 < lo -> Forall (f_cmp Cle (Znth (lo - 1) bl)) (sublist lo N bl);
+   hi + 1 < N -> Forall (f_cmp Cge (Znth (hi + 1) bl))  (sublist 0 (hi + 1) bl))
+   LOCAL (temp _left_ptr (dnth base left);
+   temp _right_ptr (dnth base right);
+   temp _mid (dnth base mid); temp _lo (dnth base lo);
+   temp _hi (dnth base hi))
+   SEP (data_at Ews (tarray tdouble N) bl base))
+ break:
+  (EX left:Z,
+   PROP (
+   lo < left <= right+1; right < hi;
+   f_cmp Cge (Znth left bl) (Znth mid bl);
+   Forall (f_cmp Cge (Znth mid bl)) (sublist lo left bl);
+   Forall (f_cmp Cle (Znth mid bl)) (sublist (right+1) (hi+1) bl);
+   Permutation al bl;
+   sorted (f_cmp Cle) (sublist 0 lo bl);
+   sorted (f_cmp Cle) (sublist (hi + 1) N bl);
+   0 < lo -> Forall (f_cmp Cle (Znth (lo - 1) bl)) (sublist lo N bl);
+   hi + 1 < N -> Forall (f_cmp Cge (Znth (hi + 1) bl))  (sublist 0 (hi + 1) bl))
+   LOCAL (temp _left_ptr (dnth base left);
+   temp _right_ptr (dnth base right);
+   temp _mid (dnth base mid); temp _lo (dnth base lo);
+   temp _hi (dnth base hi))
+   SEP (data_at Ews (tarray tdouble N) bl base)).
++
+Exists left; entailer!.
++
+clear dependent left.
+Intros left.
+pose_dnth_base left.
+forward.
+apply tc_val_tdouble_Znth; auto; omega.
+forward.
+apply tc_val_tdouble_Znth; auto; omega.
+forward_if.
+apply typed_true_cmp in H17.
+forward.
+rewrite dbase_add by (auto; rep_omega).
+Exists (left+1).
+entailer!.
+clear H27 H26 H25 H24 H23 H22 H21 H20 H19.
+split.
+split; try omega.
+assert (f_cmp Cle (Znth mid bl) (Znth (right+1) bl)).
+rewrite (sublist_split _ (right+2)) in H7 by omega.
+rewrite Forall_app in H7. destruct  H7 as [H7 _].
+rewrite sublist_one in H7 by omega. inv H7. auto.
+assert (left<>right+1);[|omega].
+intro; subst left.
+clear - H17 H19.
+apply f_cmp_swap in H17.
+eapply float_cmp_gt_le_false; eauto.
+rewrite (sublist_split _ left) by omega.
+rewrite Forall_app; split; auto.
+rewrite sublist_one by omega.
+repeat constructor; auto.
+apply f_cmp_swap in H17.
+rewrite f_cmp_ge_gt_eq; auto.
+forward.
+Exists left.
+entailer!.
+apply typed_false_cmp in H17; [ | apply Forall_Znth; auto; omega ..].
+auto.
++
+clear dependent left.
+Intros left.
+apply f_cmp_swap in H6; simpl in H6.
+forward_loop (EX right:Z,
+   PROP (
+   lo < left <= right+1; right < hi;
+   f_cmp Cle (Znth mid bl) (Znth left bl);
+   Forall (f_cmp Cge (Znth mid bl)) (sublist lo left bl);
+   Forall (f_cmp Cle (Znth mid bl)) (sublist (right+1) (hi+1) bl);
+   Permutation al bl;
+   sorted (f_cmp Cle) (sublist 0 lo bl);
+   sorted (f_cmp Cle) (sublist (hi + 1) N bl);
+   0 < lo -> Forall (f_cmp Cle (Znth (lo - 1) bl)) (sublist lo N bl);
+   hi + 1 < N -> Forall (f_cmp Cge (Znth (hi + 1) bl))  (sublist 0 (hi + 1) bl))
+   LOCAL (temp _left_ptr (dnth base left);
+   temp _right_ptr (dnth base right);
+   temp _mid (dnth base mid); temp _lo (dnth base lo);
+   temp _hi (dnth base hi))
+   SEP (data_at Ews (tarray tdouble N) bl base))
+ break:
+  (EX right:Z,
+   PROP (
+   lo < left <= right+1; right < hi;
+   f_cmp Cle (Znth mid bl) (Znth left bl);
+   f_cmp Cge (Znth mid bl) (Znth right bl);
+   Forall (f_cmp Cge (Znth mid bl)) (sublist lo left bl);
+   Forall (f_cmp Cle (Znth mid bl)) (sublist (right+1) (hi+1) bl);
+   Permutation al bl;
+   sorted (f_cmp Cle) (sublist 0 lo bl);
+   sorted (f_cmp Cle) (sublist (hi + 1) N bl);
+   0 < lo -> Forall (f_cmp Cle (Znth (lo - 1) bl)) (sublist lo N bl);
+   hi + 1 < N -> Forall (f_cmp Cge (Znth (hi + 1) bl))  (sublist 0 (hi + 1) bl))
+   LOCAL (temp _left_ptr (dnth base left);
+   temp _right_ptr (dnth base right);
+   temp _mid (dnth base mid); temp _lo (dnth base lo);
+   temp _hi (dnth base hi))
+   SEP (data_at Ews (tarray tdouble N) bl base)).
+*
+Exists right; entailer!.
+*
+clear dependent right.
+Intros right.
+pose_dnth_base right.
+forward.
+apply tc_val_tdouble_Znth; auto; omega.
+forward.
+apply tc_val_tdouble_Znth; auto; omega.
+forward_if.
+apply typed_true_cmp in H18.
+forward.
+rewrite dbase_sub by (auto; rep_omega).
+Exists (right-1).
+entailer!.
+clear H28 H27 H26 H25 H24 H23 H22 H21 H20 H19.
+split.
+split; try omega.
+rewrite Z.sub_add.
+destruct (zeq left (right+1)); try omega.
+subst left. elimtype False.
+rewrite (sublist_split lo right) in H16 by omega.
+rewrite Forall_app in H16. destruct  H16 as [_ H16].
+rewrite sublist_one in H16 by omega. inv H16.
+eapply f_cmp_lt_ge_false; eauto.
+rewrite Z.sub_add.
+rewrite (sublist_split _ (right+1)) by omega.
+rewrite Forall_app; split; auto.
+rewrite sublist_one by omega.
+repeat constructor; auto.
+rewrite f_cmp_le_lt_eq; auto.
+forward.
+Exists right.
+entailer!.
+apply typed_false_cmp in H18; [ | apply Forall_Znth; auto; omega ..].
+auto.
+*
+destruct H2 as [H2 H2'].
+destruct H3 as [H3' H3].
+clear dependent right.
+Intros right.
+pose_dnth_base left.
+pose_dnth_base right.
+forward_if (EX left:Z, EX mid:Z, EX right:Z, EX bl: list val, 
+   PROP (
+   lo < left <= right+1; right < hi; lo <= mid < hi;
+   Forall (f_cmp Cge (Znth mid bl)) (sublist lo left bl);
+   Forall (f_cmp Cle (Znth mid bl)) (sublist (right+1) (hi+1) bl);
+   Permutation al bl;
+   sorted (f_cmp Cle) (sublist 0 lo bl);
+   sorted (f_cmp Cle) (sublist (hi + 1) N bl);
+   0 < lo -> Forall (f_cmp Cle (Znth (lo - 1) bl)) (sublist lo N bl);
+   hi + 1 < N -> Forall (f_cmp Cge (Znth (hi + 1) bl))  (sublist 0 (hi + 1) bl))
+   LOCAL (temp _left_ptr (dnth base left);
+   temp _right_ptr (dnth base right);
+   temp _mid (dnth base mid); temp _lo (dnth base lo);
+   temp _hi (dnth base hi))
+   SEP (data_at Ews (tarray tdouble N) bl base)).
+--
+apply test_order_dnth; auto; rep_omega.
+--
+eapply typed_true_pp in H20; eauto; simpl in H20.
+assert (lo < left < right) by omega; clear H20 H4.
+pose (bl' := swap_in_list right left bl).
+apply semax_seq' with
+ (PROP ()
+   LOCAL (temp _left_ptr (dnth base left);
+   temp _right_ptr (dnth base right);
+   temp _mid (dnth base mid); temp _lo (dnth base lo);
+   temp _hi (dnth base hi))
+   SEP (data_at Ews (tarray tdouble N) bl' base)).
+abbreviate_semax.
+match goal with |- semax _ ?Pre _ ?Post => 
+forward_loop Pre continue:Post.(RA_normal) end;
+  [solve [auto] | | forward; apply ENTAIL_refl ].
+forward.
+apply tc_val_tdouble_Znth; auto; omega.
+forward.
+apply tc_val_tdouble_Znth; auto; omega.
+forward.
+forward.
+rewrite !def_float_f2f by (apply Forall_Znth; auto; omega).
+entailer!.
+subst MORE_COMMANDS; unfold abbreviate.
+simpl reptype in *.
+forward_if (EX mid:Z, 
+  PROP (lo <= mid < hi; 
+      f_cmp Cle (Znth left bl') (Znth mid bl');
+      Forall (f_cmp Cge (Znth mid bl')) (sublist lo left bl');
+      f_cmp Cle (Znth mid bl') (Znth right bl');
+      Forall (f_cmp Cle (Znth mid bl'))
+                  (sublist (right + 1) (hi + 1) bl'))
+   LOCAL (temp _left_ptr (dnth base left);
+   temp _right_ptr (dnth base right);
+   temp _mid (dnth base mid); temp _lo (dnth base lo);
+   temp _hi (dnth base hi))
+   SEP (data_at Ews (tarray tdouble N) bl' base)).
+++
+apply test_eq_dnth; try rep_omega; auto.
+++
+forward.
+replace base with (dnth base 0) at 1
+ by (make_Vptr base; unfold dnth; simpl; normalize).
+rewrite dbase_add by (auto; rep_omega).
+eapply typed_true_pp in H4; eauto; simpl in H4.
+rewrite Z.add_0_l.
+Exists right.
+entailer!.
+clear H27 H26 H25 H24 H23 H22 H20.
+subst bl'.
+rewrite Znth_swap_in_list2 by omega.
+rewrite Znth_swap_in_list1 by omega.
+split; [ | split3].
+apply f_cmp_swap in H7; auto.
+rewrite sublist_swap_in_list by omega; auto.
+rewrite f_cmp_le_lt_eq. right.
+apply float_cmp_eq_refl. apply Forall_Znth; auto; omega.
+rewrite sublist_swap_in_list by omega; auto.
+++
+eapply typed_false_pp in H4; eauto; simpl in H4.
+forward_if.
+**
+apply test_eq_dnth; try rep_omega; auto.
+**
+eapply typed_true_pp in H20; eauto; simpl in H20.
+forward.
+replace base with (dnth base 0) at 1
+ by (make_Vptr base; unfold dnth; simpl; normalize).
+rewrite dbase_add by (auto; rep_omega).
+rewrite Z.add_0_l.
+Exists left.
+entailer!.
+clear H28 H27 H26 H25 H24 H23 H22.
+subst bl'.
+rewrite Znth_swap_in_list2 by omega.
+rewrite Znth_swap_in_list1 by omega.
+split; [ | split3].
+apply f_cmp_swap in H7; auto.
+rewrite sublist_swap_in_list by omega; auto.
+auto.
+rewrite sublist_swap_in_list by omega; auto.
+**
+forward.
+eapply typed_false_pp in H20; eauto; simpl in H20.
+Exists mid.
+entailer!.
+clear H29 H28 H27 H26 H25 H24 H23 H22.
+subst bl'.
+rewrite Znth_swap_in_list2 by omega.
+rewrite Znth_swap_in_list1 by omega.
+rewrite Znth_swap_in_list_other by omega.
+split; [ | split3].
+apply f_cmp_swap in H7; auto.
+rewrite sublist_swap_in_list by omega; auto.
+auto.
+rewrite sublist_swap_in_list by omega; auto.
+++
+clear dependent mid.
+Intros mid.
+forward.
+forward.
+rewrite dbase_sub by (auto; rep_omega).
+rewrite dbase_add by (auto; rep_omega).
+Exists (left+1) (right-1) mid bl'.
+entailer!.
+clear H27 H26 H25 H24 H23 H22 H20 H17.
+split.
+split; try omega.
+
+subst bl'.
+
+
+forward.
+
+auto.
+
+
+
+
+Admitted.
+
+Lemma body_quicksort_while_part2:
+forall (Espec : OracleKind) (base : val) (al : list val) 
+  (lo mid hi : Z) (bl : list val),
+Forall def_float al ->
+let N := Zlength al in
+0 < N <= Z.min Int.max_signed (Ptrofs.max_signed / 8) ->
+isptr base ->
+0 <= lo <= mid ->
+mid < hi < N ->
+f_cmp Cle (Znth lo bl) (Znth mid bl) ->
+f_cmp Cle (Znth mid bl) (Znth hi bl) ->
+Permutation al bl ->
+sorted (f_cmp Cle) (sublist 0 lo bl) ->
+sorted (f_cmp Cle) (sublist (hi + 1) N bl) ->
+(0 < lo ->
+ Forall (f_cmp Cle (Znth (lo - 1) bl)) (sublist lo N bl)) ->
+(hi + 1 < N ->
+ Forall (f_cmp Cge (Znth (hi + 1) bl))
+   (sublist 0 (hi + 1) bl)) ->
+semax (func_tycontext f_quicksort Vprog Gprog [])
+  (PROP ( )
+   LOCAL (temp _mid (dnth base mid); temp _lo (dnth base lo);
+   temp _hi (dnth base hi))
+   SEP (data_at Ews (tarray tdouble N) bl base))
+  quicksort_while_body_part2
+  (normal_ret_assert
+     (EX a : Z * Z * list val,
+      PROP (0 <= fst (fst a) < N; 0 <= snd (fst a) < N;
+      Permutation al (snd a);
+      sorted (f_cmp Cle) (sublist 0 (fst (fst a)) (snd a));
+      sorted (f_cmp Cle)
+        (sublist (snd (fst a) + 1) N (snd a));
+      0 < fst (fst a) ->
+      Forall (f_cmp Cle (Znth (fst (fst a) - 1) (snd a)))
+        (sublist (fst (fst a)) N (snd a));
+      snd (fst a) + 1 < N ->
+      Forall (f_cmp Cge (Znth (snd (fst a) + 1) (snd a)))
+        (sublist 0 (snd (fst a) + 1) (snd a));
+      fst (fst a) <= snd (fst a) + 1)
+      LOCAL (temp _lo (dnth base (fst (fst a)));
+      temp _hi (dnth base (snd (fst a))))
+      SEP (data_at Ews (tarray tdouble N) (snd a) base))%assert).
+Proof.
+intros.
+set (s := quicksort_while_body_part2); hnf in s; subst s.
+abbreviate_semax.
+set (M := Z.min _ _) in H0; compute in M; subst M.
+pose_dnth_base lo.
+pose_dnth_base mid.
+pose_dnth_base hi.
+pose proof (Permutation_Zlength H6).
+forward.
+forward.
+rewrite dbase_add by (auto; rep_omega).
+rewrite dbase_sub by (auto; rep_omega).
+apply f_cmp_swap in H4; simpl in H4.
+eapply semax_seq'.
+apply forward_quicksort_do_loop; auto.
+
+
+
+
+
+Admitted.
+
+Lemma calculate_midpoint:
+  forall N base lo hi,
+0 < N <= 268435455 ->
+isptr base ->
+0 <= lo < N ->
+0 <= hi < N ->
+lo < hi ->
+force_val
+  (sem_binary_operation' Oadd (tptr tdouble) tint
+     (dnth base lo)
+     (eval_binop Oshr tint tint
+        (eval_binop Osub (tptr tdouble) (tptr tdouble)
+           (dnth base hi) (dnth base lo)) 
+        (Vint (Int.repr 1)))) = dnth base (lo + (hi - lo) / 2).
+Proof.
+intros.
+ symmetry.
+ simpl. unfold dnth, sem_shift_ii, sem_sub_pp, sem_add_ptr_int. simpl.
+    unfold sem_add_ptr_int, Cop.sem_add_ptr_int. simpl.
+    make_Vptr base; simpl. rewrite if_true by auto. simpl.
+    f_equal. rewrite Ptrofs.add_assoc. f_equal.
+    normalize. f_equal.
+    rewrite <- Z.mul_add_distr_l. f_equal.
+    unfold Int.shr.
+    rewrite !(Ptrofs.add_commut i), Ptrofs.sub_shifted.
+    normalize.
+    unfold Ptrofs.divs. normalize.
+    rewrite <- Z.mul_sub_distr_l.
+    rewrite (Int.signed_repr hi) by rep_omega.
+    rewrite (Int.signed_repr lo) by rep_omega.
+    rewrite (Ptrofs.signed_repr 8) by rep_omega.
+    rewrite (Ptrofs.signed_repr) by rep_omega.
+    rewrite Z.mul_comm, Z.quot_mul by omega.
+    rewrite Int.signed_repr. f_equal.
+    rewrite (Int.signed_repr (hi-lo)) by rep_omega.
+    rewrite Z.shiftr_div_pow2 by omega. change (2^1) with 2.
+    rewrite Int.signed_repr. auto.
+    split.
+    assert (0 <= (hi-lo)/2); [|rep_omega].
+    apply Z.div_pos; rep_omega.
+    apply Z.div_le_upper_bound; rep_omega.
+    split.
+    assert (0 <= (hi-lo)/2); [|rep_omega].
+    apply Z.div_pos; rep_omega.
+    pose proof (mid_in_range lo hi); rep_omega.
+Qed.
+
+Lemma body_quicksort_while:
+forall (Espec : OracleKind) (base : val) (al : list val) 
+  (lo hi : Z) (bl : list val),
+Forall def_float al ->
+let N := Zlength al in
+0 < N <= Z.min Int.max_signed (Ptrofs.max_signed/8) ->
+isptr base ->
+0 <= lo < N ->
+0 <= hi < N ->
+Permutation al bl ->
+sorted (f_cmp Cle) (sublist 0 lo bl) ->
+sorted (f_cmp Cle) (sublist (hi + 1) N bl) ->
+(0 < lo -> Forall (f_cmp Cle (Znth (lo - 1) bl)) (sublist lo N bl)) ->
+(hi + 1 < N ->
+ Forall (f_cmp Cge (Znth (hi + 1) bl)) (sublist 0 (hi + 1) bl)) ->
+lo < hi ->
+lo <= hi+1 ->
+semax (func_tycontext f_quicksort Vprog Gprog [])
+  (PROP ( )
+   LOCAL (temp _lo (dnth base lo); temp _hi (dnth base hi))
+   SEP (data_at Ews (tarray tdouble N) bl base)) 
+  quicksort_while_body
+  (normal_ret_assert
+     (EX a : Z * Z * list val,
+      PROP (0 <= fst (fst a) < N; 0 <= snd (fst a) < N;
+      Permutation al (snd a);
+      sorted (f_cmp Cle) (sublist 0 (fst (fst a)) (snd a));
+      sorted (f_cmp Cle) (sublist (snd (fst a) + 1) N (snd a));
+      0 < fst (fst a) ->
+      Forall (f_cmp Cle (Znth (fst (fst a) - 1) (snd a)))
+        (sublist (fst (fst a)) N (snd a));
+      snd (fst a) + 1 < N ->
+      Forall (f_cmp Cge (Znth (snd (fst a) + 1) (snd a)))
+        (sublist 0 (snd (fst a) + 1) (snd a));
+      fst (fst a) <= snd (fst a) + 1)
+      LOCAL (temp _lo (dnth base (fst (fst a)));
+      temp _hi (dnth base (snd (fst a))))
+      SEP (data_at Ews (tarray tdouble N) (snd a) base))).
+Proof.
+intros.
+abbreviate_semax.
+set (M := Z.min _ _) in H0.
+compute in M. subst M.
+assert (Hdef_bl: Forall def_float bl) by (apply Forall_perm with al; auto).
+unfold quicksort_while_body.
+simpl.
+abbreviate_semax.
+forward.
+entailer!.
+auto.
+rewrite (calculate_midpoint N) by assumption.
+pose proof (mid_in_range lo hi). spec H11; [omega|].
+forget (lo+(hi-lo)/2) as mid.
+pose_dnth_base mid.
+assert (Hlen := Permutation_Zlength H4).
+forward.
+apply tc_val_tdouble_Znth; auto; omega.
+pose_dnth_base lo.
+forward.
+apply tc_val_tdouble_Znth; auto; omega.
+forward_if (EX bl: list val, 
+   PROP (f_cmp Cle (Znth lo bl) (Znth mid bl); Permutation al bl;
+   sorted (f_cmp Cle) (sublist 0 lo bl);
+   sorted (f_cmp Cle) (sublist (hi + 1) N bl);
+   0 < lo -> Forall (f_cmp Cle (Znth (lo - 1) bl)) (sublist lo N bl);
+   hi + 1 < N -> Forall (f_cmp Cge (Znth (hi + 1) bl))  (sublist 0 (hi + 1) bl))
+   LOCAL (temp _mid (dnth base mid); temp _lo (dnth base lo);
+   temp _hi (dnth base hi))
+   SEP (data_at Ews (tarray tdouble N) bl base)).
+- (* then-clause *)
+match goal with |- semax _ ?Pre _ ?Post => 
+forward_loop Pre continue:Post.(RA_normal) end;
+  [solve [auto] | | forward; apply ENTAIL_refl ].
+apply typed_true_cmp in H14.
+assert (lo<mid). {
+ destruct (zeq lo mid); try omega.
+ clear - H14 e. subst lo. apply f_lt_irrefl in H14. contradiction.
+}
+forward.
+forward.
+forward.
+forward.
+rewrite !def_float_f2f by (apply Forall_Znth; auto; omega).
+change (upd_Znth lo _ _) with (swap_in_list lo mid bl).
+Exists (swap_in_list lo mid bl).
+entailer!.
+clear H22 H21 H20 H19 H18.
+autorewrite with sublist.
+split.
+rewrite Znth_swap_in_list1 by omega.
+rewrite Znth_swap_in_list2 by omega.
+rewrite f_cmp_le_lt_eq. auto.
+split.
+eapply Permutation_trans; [eassumption| apply Permutation_swap2; omega].
+rewrite !sublist_swap_in_list by omega.
+split3; auto.
+split; intro.
++
+rewrite Znth_swap_in_list_other by omega.
+eapply Forall_perm; [ | apply (H7 H18)].
+rewrite sublist_swap_in_list' by omega.
+apply Permutation_swap2; try list_solve.
++
+rewrite Znth_swap_in_list_other by omega.
+eapply Forall_perm; [ | apply (H8 H18)].
+rewrite sublist_swap_in_list' by omega.
+apply Permutation_swap2; try list_solve.
+-
+forward.
+Exists bl.
+entailer!.
+apply typed_false_cmp in H14.
+simpl in H14.
+apply f_cmp_swap in H14. auto.
+apply Forall_Znth; auto; omega.
+apply Forall_Znth; auto; omega.
+-
+clear dependent bl.
+Intros bl.
+assert (Hdef_bl: Forall def_float bl) by (apply Forall_perm with al; auto).
+pose proof (Permutation_Zlength H5).
+pose_dnth_base hi.
+forward.
+apply tc_val_tdouble_Znth; auto; omega.
+forward.
+apply tc_val_tdouble_Znth; auto; omega.
+forward_if (EX bl: list val, 
+   PROP (f_cmp Cle (Znth lo bl) (Znth mid bl); 
+             f_cmp Cle (Znth mid bl) (Znth hi bl); 
+             Permutation al bl;
+   sorted (f_cmp Cle) (sublist 0 lo bl);
+   sorted (f_cmp Cle) (sublist (hi + 1) N bl);
+   0 < lo -> Forall (f_cmp Cle (Znth (lo - 1) bl)) (sublist lo N bl);
+   hi + 1 < N -> Forall (f_cmp Cge (Znth (hi + 1) bl))  (sublist 0 (hi + 1) bl))
+   LOCAL (temp _mid (dnth base mid); temp _lo (dnth base lo);
+   temp _hi (dnth base hi))
+   SEP (data_at Ews (tarray tdouble N) bl base)).
++
+apply typed_true_cmp in H17.
+apply semax_seq' with (EX bl: list val, 
+   PROP (f_cmp Cle (Znth mid bl) (Znth hi bl); 
+             f_cmp Cle (Znth lo bl) (Znth mid bl) \/
+             f_cmp Cle (Znth lo bl) (Znth hi bl);
+             Permutation al bl;
+   sorted (f_cmp Cle) (sublist 0 lo bl);
+   sorted (f_cmp Cle) (sublist (hi + 1) N bl);
+   0 < lo -> Forall (f_cmp Cle (Znth (lo - 1) bl)) (sublist lo N bl);
+   hi + 1 < N -> Forall (f_cmp Cge (Znth (hi + 1) bl))  (sublist 0 (hi + 1) bl))
+   LOCAL (temp _mid (dnth base mid); temp _lo (dnth base lo);
+   temp _hi (dnth base hi))
+   SEP (data_at Ews (tarray tdouble N) bl base)).
+*
+abbreviate_semax.
+match goal with |- semax _ ?Pre _ ?Post => 
+forward_loop Pre continue:Post.(RA_normal) end;
+  [solve [auto] | | forward; apply ENTAIL_refl ].
+forward.
+forward.
+forward.
+forward.
+rewrite !def_float_f2f by (apply Forall_Znth; auto; omega).
+Exists (swap_in_list hi mid bl).
+entailer!.
+clear H24 H23 H22 H21 H20 H19 H18.
+split3.
+rewrite Znth_swap_in_list1 by omega.
+rewrite Znth_swap_in_list2 by omega.
+rewrite f_cmp_le_lt_eq. auto.
+rewrite Znth_swap_in_list1 by omega.
+rewrite Znth_swap_in_list2 by omega.
+destruct (zeq lo mid).
+subst.
+rewrite Znth_swap_in_list2 by omega.
+left.
+apply f_le_refl; auto. apply Forall_Znth; auto; omega.
+rewrite Znth_swap_in_list_other by omega.
+auto.
+split3; [ | | split]; auto.
+eapply Permutation_trans; [eassumption| ].
+apply Permutation_swap2; omega.
+rewrite sublist_swap_in_list by omega; auto.
+rewrite sublist_swap_in_list by omega; auto.
+split; intro.
+rewrite Znth_swap_in_list_other by omega.
+eapply Forall_perm; try apply (H8 H18).
+rewrite sublist_swap_in_list' by omega.
+apply Permutation_swap2; try list_solve.
+rewrite Znth_swap_in_list_other by omega.
+eapply Forall_perm; try apply (H14 H18).
+rewrite sublist_swap_in_list' by omega.
+apply Permutation_swap2; try list_solve.
+*
+clear dependent bl.
+Intros bl.
+rename H5 into H4'.
+rename H6 into H5. rename H7 into H6. rename H8 into H7.
+assert (Hdef_bl: Forall def_float bl) by (apply Forall_perm with al; auto).
+pose proof (Permutation_Zlength H5).
+abbreviate_semax.
+forward.
+apply tc_val_tdouble_Znth; auto; omega.
+forward.
+apply tc_val_tdouble_Znth; auto; omega.
+forward_if.
+--
+apply typed_true_cmp in H17.
+match goal with |- semax _ ?Pre _ ?Post => 
+forward_loop Pre continue:Post.(RA_normal) end;
+  [solve [auto] | | forward; apply ENTAIL_refl ].
+forward.
+forward.
+forward.
+forward.
+rewrite !def_float_f2f by (apply Forall_Znth; auto; omega).
+Exists (swap_in_list lo mid bl).
+entailer!.
+clear H24 H23 H22 H21 H20 H18 H19.
+assert (lo<mid). {
+ destruct (zeq lo mid); try omega.
+ clear - H17 e. subst lo. apply f_lt_irrefl in H17. contradiction.
+}
+rewrite Znth_swap_in_list1 by omega.
+rewrite Znth_swap_in_list2 by omega.
+rewrite Znth_swap_in_list_other by omega.
+split3; auto.
+rewrite f_cmp_le_lt_eq. auto.
+destruct H4'; auto.
+eapply f_cmp_le_trans; try eassumption.
+split3; [ | | split]; auto.
+eapply Permutation_trans; [eassumption| ].
+apply Permutation_swap2; try omega.
+rewrite sublist_swap_in_list by omega; auto.
+rewrite sublist_swap_in_list by omega; auto.
+split; intro.
+++
+rewrite Znth_swap_in_list_other by omega.
+eapply Forall_perm; try apply (H14 H19).
+rewrite sublist_swap_in_list' by omega.
+apply Permutation_swap2; try list_solve.
+++
+rewrite Znth_swap_in_list_other by omega.
+eapply Forall_perm; try apply (H15 H19).
+rewrite sublist_swap_in_list' by omega.
+apply Permutation_swap2; try list_solve.
+--
+forward.
+Exists bl.
+entailer!.
+apply typed_false_cmp in H17.
+simpl in H17.
+apply f_cmp_swap in H17. auto.
+apply Forall_Znth; auto; omega.
+apply Forall_Znth; auto; omega.
++
+forward.
+Exists bl.
+entailer!.
+apply typed_false_cmp in H17.
+simpl in H17.
+apply f_cmp_swap in H17. auto.
+apply Forall_Znth; auto; omega.
+apply Forall_Znth; auto; omega.
++
+clear dependent bl.
+Intros bl.
+apply body_quicksort_while_part2; auto; omega.
+Qed.
+
+Lemma body_quicksort:  semax_body Vprog Gprog f_quicksort quicksort_spec.
+Proof.
+start_function.
+rename H0 into H0''.
+assert (H0' := Z.min_glb_r _ _ _ H0'').
+assert (H0 := Z.min_glb_l _ _ _ H0'').
+forward_if.
+forward.
+Exists al.
+entailer!.
+destruct al; autorewrite with sublist in H2; try rep_omega.
+constructor.
+assert (0 < N <= Int.max_signed) by rep_omega.
+clear H0 H2.
+assert_PROP (isptr base) by entailer!.
+forward.
+forward.
+replace  (force_val
+               (sem_binary_operation' Osub (tptr tdouble) tint
+                  (eval_binop Oadd (tptr tdouble) tint base
+                     (Vint (Int.repr N))) (Vint (Int.repr 1))))
+  with (dnth base (N-1)).
+2:{
+  make_Vptr base.
+  unfold dnth.
+  simpl. f_equal. rewrite ptrofs_of_ints_unfold.
+  rewrite Ptrofs.sub_add_opp.
+  normalize.
+  rewrite Ptrofs.add_assoc. f_equal.
+  change (Ptrofs.neg (Ptrofs.repr 8)) with (Ptrofs.repr (-8)).
+  normalize. f_equal. omega.
+}
+deadvars!.
+subst N.
+set (N := Zlength al) in *.
+forward_while (EX lo:Z, EX hi:Z, EX bl: list val,
+                       PROP(0 <= lo < N; 0 <= hi < N;Permutation al bl;
+                                sorted (f_cmp Cle) (sublist 0 lo bl);
+                                sorted (f_cmp Cle) (sublist (hi+1) N bl);
+                                0<lo -> Forall (f_cmp Cle (Znth (lo-1) bl))
+                                                    (sublist lo N bl);
+                                hi+1<N -> Forall (f_cmp Cge (Znth (hi+1) bl))
+                                                    (sublist 0 (hi+1) bl);
+                                lo <= hi+1)
+                       LOCAL(temp _lo (dnth base lo); temp _hi (dnth base hi))
+                       SEP(data_at Ews (tarray tdouble N) bl base)).
+-
+Exists 0 (N-1) al.
+entailer!.
+autorewrite with sublist.
+split3.
+constructor.
+constructor.
+unfold dnth. clear - H0. make_Vptr base. simpl. f_equal.
+  rewrite ptrofs_of_ints_unfold. normalize.
+-
+entailer!.
+assert (0 <= lo <= Zlength al) by omega.
+assert (0 <= hi <= Zlength al) by omega.
+auto with valid_pointer.
+-
+pose_dnth_base lo. rename H10 into Hlo.
+pose_dnth_base hi. rename H10 into Hhi.
+rewrite <- (force_sem_cmp_pp Clt) in HRE
+  by (apply isptr_dnth; auto).
+eapply typed_true_pp with (N:=N) in HRE; 
+  eauto; try split; try assumption; try omega; simpl in HRE.
+rename HRE into H10.
+change Delta with (func_tycontext f_quicksort Vprog Gprog nil).
+change (Ssequence _ _) with quicksort_while_body.
+make_sequential.
+subst POSTCONDITION; unfold abbreviate.
+autorewrite with ret_assert.
+apply body_quicksort_while; auto.
+split. omega.
+apply Z.min_glb; auto. omega.
+-
+forward.
+assert_PROP (lo >= hi). {
+entailer!.
+unfold compare_pp, dnth in HRE.
+destruct base; simpl in HRE; try solve [inv HRE].
+rewrite if_true in HRE by auto.
+rewrite !ptrofs_of_ints_unfold in HRE.
+normalize in HRE.
+unfold Ptrofs.ltu in HRE.
+destruct (zlt _ _) in HRE; inv HRE.
+rewrite <- H13 in *.
+clear H13 al H1 H4 H13 H9 H10 H7 H8 H5 H6 H0.
+rewrite <- (Ptrofs.repr_unsigned i) in g.
+normalize in g.
+destruct H12 as [? [? [? [? ?]]]].
+red in H4.
+simpl  sizeof in H4.
+rewrite Z.max_r in H4 by rep_omega.
+rewrite !Ptrofs.unsigned_repr in g by rep_omega.
+omega.
+} clear HRE.
+Exists bl.
+entailer!.
+assert (lo=hi \/ lo=hi+1) by omega.
+assert (Zlength al = Zlength bl) 
+  by (rewrite !Zlength_correct; f_equal; apply Permutation_length; auto).
+rewrite H17 in *. 
+assert (Hdef_bl: Forall def_float bl). {eapply Forall_perm; try eassumption. }
+clear - H16 H7 H8 H5 H6 H H2 Hdef_bl.
+destruct H16; subst.
++
+assert (hi=0 \/ 0<hi) by omega.
+destruct H0.
+ *
+subst.
+autorewrite with sublist in *.
+destruct (zlt 1 (Zlength bl)).
+specialize (H8 l).
+rewrite sublist_one in H8 by omega.
+inv H8.
+rewrite <- (sublist_same 0 (Zlength bl) bl) by omega.
+rewrite (sublist_split _ 1) by omega.
+rewrite sublist_one by omega.
+apply sorted_app with (Znth 1 bl); auto.
+apply f_cmp_le_trans.
+constructor.
+constructor.
+apply (f_cmp_swap _ _ _ H3).
+constructor.
+{
+ clear - H6 l Hdef_bl.
+ destruct bl. inv l.
+ inv Hdef_bl. clear H1.
+ rewrite Zlength_cons in *. change (v::bl) with ([v]++bl) in *.
+ autorewrite with sublist in *.
+ assert (0 < Zlength bl) by omega. clear l.
+ revert H H2; induction H6; intros. 
+ constructor. repeat constructor. inv H2.  apply f_le_refl; auto.
+ change (Znth 0 (x::y::l)) with x. inv H2.
+ constructor.  apply f_le_refl; auto.
+ spec IHsorted.
+ rewrite Zlength_cons. rep_omega.
+ spec IHsorted; auto.
+ change (Znth 0 (y::l)) with y in IHsorted.
+ clear - H IHsorted.
+ forget (y::l) as zl.
+ induction IHsorted. constructor. constructor; auto.
+ eapply f_cmp_le_trans; eassumption.
+}
+destruct bl.
+constructor.
+destruct bl.
+constructor.
+rewrite !Zlength_cons in g.
+rep_omega.
+ *
+specialize (H7 H0).
+destruct (zlt (hi+1) (Zlength bl)).
+2:{ assert (hi=Zlength bl \/ hi+1 = Zlength bl) by omega.
+    destruct H1. subst. autorewrite with sublist in *. auto.
+    autorewrite with sublist in *.
+    clear g H6 H2 H H8.
+    rewrite sublist_one in H7 by omega. inv H7. clear H4.
+    rewrite (sublist_split 0 (hi-1)) in H5 by omega.
+    rewrite (sublist_one (hi-1)) in H5 by omega.
+    rewrite <- (sublist_same 0 (hi+1)) by omega.
+    rewrite (sublist_split 0 (hi-1)) by omega.
+    rewrite (sublist_split (hi-1) hi) by omega.
+    rewrite (sublist_one (hi-1)) by omega.
+    rewrite (sublist_one hi) by omega.
+    clear - H5 H3.
+    induction (sublist 0 (hi-1) bl). constructor; auto. constructor; auto.
+    inv H5. destruct l; inv H1. destruct l; inv H0.
+    simpl in IHl. spec IHl; auto. constructor; auto.
+    simpl in *. spec IHl; auto. constructor; auto.
+}
+specialize (H8 l).
+rewrite <- (sublist_same 0 (Zlength bl) bl) by omega.
+rewrite (sublist_split 0 (hi-1)) by omega.
+apply sorted_app with (Znth (hi-1) bl); auto.
+apply f_cmp_le_trans.
+{
+clear - H0 l H5.
+rewrite (sublist_split 0 (hi-1)) in H5 by list_solve.
+forget (sublist 0 (hi - 1) bl) as al.
+induction al. constructor.
+simpl in H5.
+inv H5.
+destruct al. constructor.
+inv H2.
+destruct al; inv H1.
+constructor.
+constructor; auto.
+}
+{
+rewrite (sublist_split (hi-1) hi) by rep_omega.
+rewrite sublist_one by omega.
+rewrite (sublist_split hi (hi+1)) by rep_omega.
+rewrite sublist_one by omega.
+simpl.
+constructor.
+rewrite (sublist_split hi (hi+1)) in H7 by rep_omega.
+rewrite sublist_one in H7 by rep_omega.
+inv H7.
+auto.
+rewrite (sublist_split 0 (hi-1)) in H8 by omega.
+rewrite Forall_app in H8. destruct H8.
+rewrite (sublist_split _ hi) in H3 by omega.
+rewrite Forall_app in H3. destruct H3.
+rewrite sublist_one in H4 by omega.
+inv H4. clear H11.
+apply f_cmp_swap in H10. simpl in H10.
+rewrite (sublist_split _ (hi+2)) in H6|-* by omega.
+rewrite sublist_one in * by omega.
+clear - H10 H6.
+simpl in *.
+constructor; auto.
+}
+rewrite (sublist_split 0 (hi-1)) in H8 by omega.
+{
+clear - H5 H0 l Hdef_bl.
+rewrite (sublist_split 0 (hi-1)) in H5 by omega.
+rewrite (sublist_one (hi-1)) in H5 by omega.
+clear - H5.
+induction (sublist 0 (hi - 1) bl). constructor.
+inv H5. destruct l; inv H1.
+destruct l; inv H0.
+constructor; auto.
+constructor; auto.
+spec IHl; auto. inv IHl; auto.
+apply f_cmp_le_trans with v; auto.
+}
+rewrite (sublist_split _ hi) by omega.
+rewrite Forall_app. split; auto.
+rewrite sublist_one by omega. repeat constructor.
+apply f_le_refl.
+apply Forall_Znth; auto. omega.
++
+spec H7; [ omega|].
+rewrite Z.add_simpl_r in H7.
+destruct (zlt (hi+1) (Zlength bl)).
+specialize (H8 l).
+rewrite <- (sublist_same 0 (Zlength bl) bl) by omega.
+rewrite (sublist_split 0 (hi+1)) by omega.
+apply sorted_app with (Znth (hi+1) bl); auto.
+apply f_cmp_le_trans.
+eapply Forall_impl; try apply H8.
+clear; intros; apply (f_cmp_swap _ _ _ H).
+{
+clear - H6 l H2 Hdef_bl.
+rewrite (sublist_split (hi+1) (hi+2)) in H6|-* by omega.
+rewrite sublist_one in H6|-* by omega.
+induction (sublist (hi + 2) (Zlength bl) bl).
+constructor; auto.
+apply f_le_refl.
+apply Forall_Znth; try omega.
+apply Hdef_bl.
+constructor.
+apply f_le_refl.
+apply Forall_Znth; auto. omega.
+inv H6.
+spec IHl0.
+destruct l0; inv H4; constructor; auto.
+eapply f_cmp_le_trans; eassumption.
+constructor; auto.
+inv IHl0; auto.
+}
+assert (hi+1=Zlength bl) by omega.
+autorewrite with sublist in *.
+auto.
+Qed.
+
+
+
+
+
+
+
+
+
